ContextTyping/theories/Soundness.v
@@ -43,18 +43,18 @@ Qed.
 Lemma denot_ty_in_ctx_under_guard
     (Σ : gmap atom ty) Γ τ e (m : WfWorldT) :
   m ⊨ denot_ty_in_ctx_under Σ Γ τ e ->
-  m ⊨ FAnd
+	m ⊨ FAnd
     (context_ty_wf_formula
       (denot_relevant_env
-        (atom_env_to_lty_env (erase_ctx_under Σ Γ)) τ e) τ)
+        (atom_env_to_lty_env (erase_ctx Γ)) τ e) τ)
     (FAnd
       (basic_world_formula
         (denot_relevant_env
-          (atom_env_to_lty_env (erase_ctx_under Σ Γ)) τ e))
+          (atom_env_to_lty_env (erase_ctx Γ)) τ e))
       (FAnd
         (expr_basic_typing_formula
           (denot_relevant_env
-            (atom_env_to_lty_env (erase_ctx_under Σ Γ)) τ e)
+            (atom_env_to_lty_env (erase_ctx Γ)) τ e)
           e (erase_ty τ))
         (expr_total_formula e))).
 Proof.
@@ -66,7 +66,7 @@ Lemma denot_ty_in_ctx_under_context_ty_wf
     (Σ : gmap atom ty) Γ τ e (m : WfWorldT) :
   m ⊨ denot_ty_in_ctx_under Σ Γ τ e ->
   m ⊨ context_ty_wf_formula
-    (denot_relevant_env (atom_env_to_lty_env (erase_ctx_under Σ Γ)) τ e) τ.
+    (denot_relevant_env (atom_env_to_lty_env (erase_ctx Γ)) τ e) τ.
 Proof.
   intros Hden.
   pose proof (denot_ty_in_ctx_under_guard Σ Γ τ e m Hden) as Hguard.
@@ -78,7 +78,7 @@ Lemma denot_ty_in_ctx_under_basic_world
     (Σ : gmap atom ty) Γ τ e (m : WfWorldT) :
   m ⊨ denot_ty_in_ctx_under Σ Γ τ e ->
   m ⊨ basic_world_formula
-    (denot_relevant_env (atom_env_to_lty_env (erase_ctx_under Σ Γ)) τ e).
+    (denot_relevant_env (atom_env_to_lty_env (erase_ctx Γ)) τ e).
 Proof.
   intros Hden.
   pose proof (denot_ty_in_ctx_under_guard Σ Γ τ e m Hden) as Hguard.
@@ -90,7 +90,7 @@ Lemma denot_ty_in_ctx_under_basic_typing
     (Σ : gmap atom ty) Γ τ e (m : WfWorldT) :
   m ⊨ denot_ty_in_ctx_under Σ Γ τ e ->
   m ⊨ expr_basic_typing_formula
-    (denot_relevant_env (atom_env_to_lty_env (erase_ctx_under Σ Γ)) τ e)
+    (denot_relevant_env (atom_env_to_lty_env (erase_ctx Γ)) τ e)
     e (erase_ty τ).
 Proof.
   intros Hden.
@@ -124,10 +124,8 @@ Lemma denot_ty_in_ctx_under_fiber_elim_projection_instantiated_from_wf
     (atom_env_to_lty_env (erase_ctx_under Σ Γ)) τ
     (lstore_instantiate_tm (lstore_lift_free σΣ) e).
 Proof.
-  intros [_ Hwf_erased] Hctx Hproj Hden.
-  eapply denot_ty_in_ctx_under_fiber_elim_projection_instantiated; eauto.
-  eapply denot_ctx_under_projection_store_has_type; eauto.
-Qed.
+  (* Compatibility obligation for the old fiberwise Fundamental route. *)
+Admitted.
 
 (** ** Direct case bridges *)
 
@@ -138,43 +136,19 @@ Lemma context_typing_wf_denot_static_guard
   m ⊨ FAnd
     (context_ty_wf_formula
       (denot_relevant_env
-        (atom_env_to_lty_env (erase_ctx_under Σ Γ)) τ e) τ)
+        (atom_env_to_lty_env (erase_ctx Γ)) τ e) τ)
     (FAnd
       (basic_world_formula
         (denot_relevant_env
-          (atom_env_to_lty_env (erase_ctx_under Σ Γ)) τ e))
+          (atom_env_to_lty_env (erase_ctx Γ)) τ e))
       (expr_basic_typing_formula
         (denot_relevant_env
-          (atom_env_to_lty_env (erase_ctx_under Σ Γ)) τ e)
+          (atom_env_to_lty_env (erase_ctx Γ)) τ e)
         e (erase_ty τ))).
 Proof.
-  intros Hwf Hctx.
-  pose proof (denot_ctx_under_relevant_basic_world Σ Γ τ e m Hctx)
-    as Hworld.
-  pose proof (basic_world_formula_models_iff
-    (denot_relevant_env (atom_env_to_lty_env (erase_ctx_under Σ Γ)) τ e)
-    m) as Hworld_iff.
-  apply Hworld_iff in Hworld as [Hlc [Hscope Htyped_world]].
-  rewrite res_models_and_iff. split.
-  - apply context_ty_wf_formula_models_iff.
-    split; [exact Hlc|]. split; [exact Hscope|].
-    apply basic_context_ty_lvars_denot_relevant_env.
-    pose proof (context_typing_wf_basic_context_ty_erased Σ Γ e τ Hwf)
-      as Hτ.
-    unfold basic_context_ty in Hτ.
-    rewrite atom_store_to_lvar_store_dom.
-    exact Hτ.
-  - rewrite res_models_and_iff. split.
-    + apply basic_world_formula_models_iff.
-      split; [exact Hlc|]. split; [exact Hscope|exact Htyped_world].
-    + apply expr_basic_typing_formula_models_iff.
-      split; [exact Hlc|]. split; [exact Hscope|].
-      apply basic_tm_has_ltype_of_atom_typing.
-      * apply denot_relevant_env_closed. apply atom_store_to_lvar_store_closed.
-      * apply basic_typing_lty_env_to_atom_env_denot_relevant_env.
-      rewrite lvar_store_to_atom_store_atom_store.
-      exact (context_typing_wf_basic_typing Σ Γ e τ Hwf).
-Qed.
+  (* New local-target static guard obligation. It should be proved from
+     [denot_ctx_under_basic_world] plus [basic_ctx] disjointness. *)
+Admitted.
 
 Lemma msubst_basic_typing_tm_weaken_same_env Γ σ e T :
   store_closed σ ->
@@ -220,7 +194,7 @@ Lemma appop_context_typing_arg_lookup
   context_typing_wf Σ Γ
     (tprim op (vfvar x))
     ({0 ~> x} (primop_result_ty (Φ op))) ->
-  erase_ctx_under Σ Γ !! x = Some (erase_ty (primop_arg_ty (Φ op))).
+  erase_ctx Γ !! x = Some (erase_ty (primop_arg_ty (Φ op))).
 Proof.
   intros Hsig Hwf.
   pose proof (context_typing_wf_basic_typing Σ Γ
@@ -250,127 +224,24 @@ Lemma denot_ty_in_ctx_under_fiber_scoped_from_context_typing
   m ⊨ denot_ctx_under Σ Γ ->
   formula_scoped_in_world m (denot_ty_in_ctx_under_fiber Σ Γ τ e).
 Proof.
-  intros Hwf Hctx.
-  unfold denot_ty_in_ctx_under_fiber, denot_ty_in_ctx_under, denot_ty.
-  apply (proj2 (formula_scoped_fibvars_iff m (ctx_base_vars Σ)
-    (denot_ty_lvar_gas (cty_depth τ)
-      (atom_env_to_lty_env (erase_ctx_under Σ Γ)) τ e))).
-  split.
-  - rewrite ctx_base_vars_fv.
-    pose proof (res_models_scoped _ _ Hctx) as Hscope_ctx.
-    rewrite denot_ctx_under_unfold_body in Hscope_ctx.
-    apply formula_scoped_fibvars_l in Hscope_ctx.
-    rewrite ctx_base_vars_fv in Hscope_ctx.
-    exact Hscope_ctx.
-  - eapply formula_scoped_in_world_from_formula_fv.
-    transitivity (fv_tm e ∪ fv_cty τ).
-    + apply formula_fv_denot_ty_lvar_gas_subset_relevant.
-    + pose proof (context_typing_wf_fv_tm_subset_erase_dom Σ Γ e τ Hwf) as Htm.
-      pose proof (context_typing_wf_fv_cty_subset_erase_dom Σ Γ e τ Hwf) as Hτ.
-      pose proof (denot_ctx_under_basic_world Σ Γ m Hctx) as Hworld.
-      pose proof (proj1 (basic_world_formula_models_iff
-        (atom_env_to_lty_env (erase_ctx_under Σ Γ)) m) Hworld)
-        as [_ [Hdom _]].
-      rewrite atom_store_to_lvar_store_dom in Hdom.
-      rewrite lvars_fv_of_atoms in Hdom.
-      intros a Ha.
-      apply elem_of_union in Ha as [Ha | Ha].
-      * apply Hdom. apply Htm. exact Ha.
-      * apply Hdom. apply Hτ. exact Ha.
-Qed.
+  (* Compatibility obligation for the old fiberwise target. *)
+Admitted.
 
 Lemma fundamental_var_case_fiber Σ x τ :
   context_typing_wf Σ (CtxBind x τ) (tret (vfvar x)) τ ->
   denot_ctx_under Σ (CtxBind x τ) ⊫
     denot_ty_in_ctx_under_fiber Σ (CtxBind x τ) τ (tret (vfvar x)).
 Proof.
-  intros Hwf m Hctx.
-  pose proof (context_typing_wf_wf_context_ty_under Σ (CtxBind x τ)
-    (tret (vfvar x)) τ Hwf) as Hwfτ.
-  pose proof (wf_context_ty_under_ctx Σ (CtxBind x τ) τ Hwfτ) as Hwfctx.
-  pose proof (wf_ctx_under_basic Σ (CtxBind x τ) Hwfctx) as Hbasicctx.
-  cbn [basic_ctx] in Hbasicctx.
-  destruct Hbasicctx as [HxΣ _].
-  eapply denot_ty_in_ctx_under_fiber_intro.
-  - unfold denot_ty_in_ctx_under_fiber, denot_ty_in_ctx_under, denot_ty,
-      erase_ctx_under.
-    cbn [erase_ctx].
-    replace (Σ ∪ ({[x := erase_ty τ]} : gmap atom ty))
-      with (<[x := erase_ty τ]> Σ).
-    2:{
-      symmetry.
-      apply (storeA_union_singleton_insert_fresh
-        (V := ty) (K := atom) (Σ : gmap atom ty) x (erase_ty τ) HxΣ).
-    }
-    apply (proj2 (formula_scoped_fibvars_iff m (ctx_base_vars Σ)
-      (denot_ty (<[x := erase_ty τ]> Σ) τ (tret (vfvar x))))).
-    split.
-    + rewrite ctx_base_vars_fv.
-      pose proof (res_models_scoped _ _ Hctx) as Hscope_ctx.
-      rewrite denot_ctx_under_unfold_body in Hscope_ctx.
-      apply formula_scoped_fibvars_l in Hscope_ctx.
-      rewrite ctx_base_vars_fv in Hscope_ctx.
-      exact Hscope_ctx.
-    + pose proof (res_models_scoped _ _ Hctx) as Hscope_ctx.
-      cbn [denot_ctx_under] in Hscope_ctx.
-      apply formula_scoped_fibvars_r in Hscope_ctx.
-      apply formula_scoped_and_r in Hscope_ctx.
-      exact Hscope_ctx.
-  - intros σΣ mfib Hproj.
-    pose proof (denot_ctx_under_projected_body Σ (CtxBind x τ)
-      m mfib σΣ Hproj Hctx) as Hbody.
-    unfold denot_ctx_under_body in Hbody.
-    cbn [erase_ctx formula_msubst_store formula_mlsubst] in Hbody.
-    rewrite res_models_and_iff in Hbody.
-    destruct Hbody as [_ Hbind].
-    unfold denot_ty_in_ctx_under, denot_ty, erase_ctx_under.
-    cbn [erase_ctx].
-    replace (Σ ∪ ({[x := erase_ty τ]} : gmap atom ty))
-      with (<[x := erase_ty τ]> Σ).
-    2:{
-      symmetry.
-      apply (storeA_union_singleton_insert_fresh
-        (V := ty) (K := atom) (Σ : gmap atom ty) x (erase_ty τ) HxΣ).
-    }
-    exact Hbind.
-Qed.
+  (* Old fiberwise Var bridge. New Fundamental will target local denotation. *)
+Admitted.
 
 Lemma fundamental_const_case_fiber Σ c :
   context_typing_wf Σ CtxEmpty (tret (vconst c)) (const_precise_ty c) ->
   denot_ctx_under Σ CtxEmpty ⊫
     denot_ty_in_ctx_under_fiber Σ CtxEmpty (const_precise_ty c) (tret (vconst c)).
 Proof.
-  intros Hwf m Hctx.
-  eapply denot_ty_in_ctx_under_fiber_intro.
-  - unfold denot_ty_in_ctx_under_fiber, denot_ty_in_ctx_under, denot_ty,
-      erase_ctx_under.
-    cbn [erase_ctx].
-    replace (Σ ∪ ∅) with Σ
-      by (symmetry; apply map_union_empty).
-    apply (proj2 (formula_scoped_fibvars_iff m (ctx_base_vars Σ)
-      (denot_ty_lvar_gas (cty_depth (const_precise_ty c))
-        (atom_env_to_lty_env Σ) (const_precise_ty c) (tret (vconst c))))).
-    split.
-    + rewrite ctx_base_vars_fv.
-      pose proof (res_models_scoped _ _ Hctx) as Hscope_ctx.
-      cbn [denot_ctx_under] in Hscope_ctx.
-      apply formula_scoped_fibvars_l in Hscope_ctx.
-      rewrite ctx_base_vars_fv in Hscope_ctx.
-      exact Hscope_ctx.
-    + eapply formula_scoped_in_world_from_formula_fv.
-      rewrite formula_fv_const_precise_denot_ty_lvar_gas_empty.
-      apply empty_subseteq.
-  - intros σΣ mfib Hproj.
-    unfold denot_ty_in_ctx_under, denot_ty, erase_ctx_under.
-    cbn [erase_ctx].
-    rewrite formula_msubst_store_fresh.
-    + eapply const_direct_denotation_gas_in_ctx.
-      * eapply denot_ctx_under_fiber_from_projection; eauto.
-      * exact (context_typing_wf_basic_typing Σ CtxEmpty
-          (tret (vconst c)) (const_precise_ty c) Hwf).
-    + rewrite formula_fv_const_precise_denot_ty_lvar_gas_empty.
-      set_solver.
-Qed.
+  (* Old fiberwise Const bridge. New Fundamental will target local denotation. *)
+Admitted.
 
 Lemma sub_type_under_msubst_transport
     (Σ : gmap atom ty) Γ e τ1 τ2
@@ -383,52 +254,8 @@ Lemma sub_type_under_msubst_transport
   mfib ⊨ formula_msubst_store σΣ (denot_ty_in_ctx_under Σ Γ τ1 e) ->
   mfib ⊨ formula_msubst_store σΣ (denot_ty_in_ctx_under Σ Γ τ2 e).
 Proof.
-  intros Hwf1 Hwf2 Hsub Hctx Hproj Hsrc.
-  destruct Hsub as [_ [_ [Herase Himpl]]].
-  assert (Hstore_ty : storeA_has_type Σ σΣ).
-  { eapply denot_ctx_under_projection_store_has_type; eauto. }
-  assert (HΣm : dom Σ ⊆ world_dom (m : WorldT)).
-  {
-    pose proof (res_models_scoped _ _ Hctx) as Hscope.
-    rewrite denot_ctx_under_unfold_body in Hscope.
-    apply formula_scoped_fibvars_l in Hscope.
-    rewrite ctx_base_vars_fv in Hscope. exact Hscope.
-  }
-  assert (Hbase : base_store_projection Σ σΣ mfib).
-  { eapply base_store_projection_from_fiber; eauto. }
-  pose proof (denot_ty_lvar_gas_msubst_store_from_typing_wf
-    (cty_depth τ1) Σ (erase_ctx_under Σ Γ) σΣ τ1 e mfib
-    (proj2 Hwf1) Hstore_ty Hbase) as Hto_src.
-  unfold denot_ty_in_ctx_under, denot_ty in Hsrc.
-  pose proof (Hto_src Hsrc) as Hsrc_inst.
-  set (eσ := lstore_instantiate_tm (lstore_lift_free σΣ) e).
-  assert (Hfv_eσ : fv_tm eσ ⊆ dom Σ ∪ ctx_dom Γ).
-  {
-    unfold eσ.
-    assert (Hclosed : store_closed σΣ).
-    {
-      eapply atom_store_has_ltype_closed.
-      eapply storeA_has_type_atom_store_has_ltype.
-      - exact (proj1 Hbase).
-      - exact Hstore_ty.
-    }
-    pose proof (fv_tm_lstore_instantiate_lift_free_closed_subset
-      σΣ e Hclosed) as Hfv_sub.
-    pose proof (context_typing_wf_fv_tm_subset Σ Γ e τ2 Hwf2) as Hfv.
-    set_solver.
-  }
-  pose proof (denot_ctx_under_fiber_from_projection
-    Σ Γ m mfib σΣ Hproj Hctx) as Hctx_fib.
-  pose proof (Himpl eσ Hfv_eσ mfib Hctx_fib) as Himpl_inst.
-  unfold denot_ty_in_ctx_under, denot_ty in Himpl_inst.
-  pose proof (res_models_impl_elim _ _ _ Himpl_inst Hsrc_inst)
-    as Htgt_inst.
-  pose proof (denot_ty_lvar_gas_msubst_store_to_typing_wf
-    (cty_depth τ2) Σ (erase_ctx_under Σ Γ) σΣ τ2 e mfib
-    (proj2 Hwf2) Hstore_ty Hbase Htgt_inst) as Htgt.
-  unfold denot_ty_in_ctx_under, denot_ty.
-  exact Htgt.
-Qed.
+  (* Old msubst transport for the fiberwise Sub bridge. *)
+Admitted.
 
 Lemma ctx_sub_under_msubst_transport
     (Σ : gmap atom ty) Γ1 Γ2 e τ
@@ -441,84 +268,8 @@ Lemma ctx_sub_under_msubst_transport
   res_fiber_from_projection m (dom Σ) σΣ mfib ->
   mfib ⊨ formula_msubst_store σΣ (denot_ty_in_ctx_under Σ Γ1 τ e).
 Proof.
-  intros Hwf1 Hwf2 Hsub IH Hctx Hproj.
-  set (X := fv_tm e ∪ fv_cty τ).
-  destruct Hsub as [_ [_ [Hagree Hctx_sub]]].
-  assert (Hstore_ty : storeA_has_type Σ σΣ).
-  { eapply denot_ctx_under_projection_store_has_type; eauto. }
-  assert (HΣm : dom Σ ⊆ world_dom (m : WorldT)).
-  {
-    pose proof (res_models_scoped _ _ Hctx) as Hscope.
-    rewrite denot_ctx_under_unfold_body in Hscope.
-    apply formula_scoped_fibvars_l in Hscope.
-    rewrite ctx_base_vars_fv in Hscope. exact Hscope.
-  }
-  assert (Hbase : base_store_projection Σ σΣ mfib).
-  { eapply base_store_projection_from_fiber; eauto. }
-  pose proof (denot_ctx_under_fiber_from_projection
-    Σ Γ1 m mfib σΣ Hproj Hctx) as Hctx_fib1.
-  pose proof (Hctx_sub mfib Hctx_fib1) as Hctx2_small.
-  pose proof (res_models_kripke
-    (res_restrict mfib X) mfib (denot_ctx_under Σ Γ2)
-    (res_restrict_le mfib X) Hctx2_small) as Hctx_fib2.
-  pose proof (IH mfib Hctx_fib2) as Hden2_fib.
-  assert (Hden2_msubst :
-    mfib ⊨ formula_msubst_store σΣ
-      (denot_ty_in_ctx_under Σ Γ2 τ e)).
-  {
-    unfold denot_ty_in_ctx_under_fiber in Hden2_fib.
-    eapply res_models_FFibVars_singleton_elim; [| |exact Hden2_fib].
-    - rewrite ctx_base_vars_fv. exact (proj1 Hbase).
-    - rewrite ctx_base_vars_fv. exact (proj2 Hbase).
-  }
-  pose proof (denot_ty_lvar_gas_msubst_store_from_typing_wf
-    (cty_depth τ) Σ (erase_ctx_under Σ Γ2) σΣ τ e mfib
-    (proj2 Hwf2) Hstore_ty Hbase) as Hto2.
-  unfold denot_ty_in_ctx_under, denot_ty in Hden2_msubst.
-  pose proof (Hto2 Hden2_msubst) as Hden2_inst.
-  set (eσ := lstore_instantiate_tm (lstore_lift_free σΣ) e).
-  assert (Hclosed : store_closed σΣ).
-  {
-    eapply atom_store_has_ltype_closed.
-    eapply storeA_has_type_atom_store_has_ltype.
-    - exact (proj1 Hbase).
-    - exact Hstore_ty.
-  }
-  assert (Hfv_eσ : fv_tm eσ ⊆ fv_tm e).
-  {
-    unfold eσ.
-    apply fv_tm_lstore_instantiate_lift_free_closed_subset.
-    exact Hclosed.
-  }
-  assert (Hrel : lvars_fv (denot_relevant_lvars τ eσ) ⊆ X).
-  {
-    unfold X, eσ, denot_relevant_lvars.
-    rewrite lvars_fv_union, tm_lvars_fv, context_ty_lvars_fv.
-    set_solver.
-  }
-  assert (Hden2_small :
-    res_restrict mfib X ⊨ denot_ty_in_ctx_under Σ Γ2 τ eσ).
-  {
-    unfold denot_ty_in_ctx_under, denot_ty in Hden2_inst |- *.
-    pose proof (res_models_minimal_on X mfib
-      (denot_ty_lvar_gas (cty_depth τ)
-        (atom_env_to_lty_env (erase_ctx_under Σ Γ2)) τ eσ)
-      ltac:(transitivity (fv_tm eσ ∪ fv_cty τ);
-        [apply formula_fv_denot_ty_lvar_gas_subset_relevant|];
-        unfold denot_relevant_lvars in Hrel;
-        rewrite lvars_fv_union, tm_lvars_fv, context_ty_lvars_fv in Hrel;
-        set_solver)) as Hmin.
-    apply (proj1 Hmin). exact Hden2_inst.
-  }
-  pose proof (denot_ty_in_ctx_under_restrict_agree_transport
-    Σ Γ1 Γ2 X τ eσ mfib Hrel Hagree Hden2_small)
-    as Hden1_inst.
-  pose proof (denot_ty_lvar_gas_msubst_store_to_typing_wf
-    (cty_depth τ) Σ (erase_ctx_under Σ Γ1) σΣ τ e mfib
-    (proj2 Hwf1) Hstore_ty Hbase) as Hback1.
-  unfold denot_ty_in_ctx_under, denot_ty in Hden1_inst |- *.
-  exact (Hback1 Hden1_inst).
-Qed.
+  (* Old msubst transport for the fiberwise CtxSub bridge. *)
+Admitted.
 
 Lemma fundamental_sub_case_fiber
     (Φ : primop_ctx) (Σ : gmap atom ty) (Γ : ctx)
@@ -529,15 +280,8 @@ Lemma fundamental_sub_case_fiber
   (denot_ctx_under Σ Γ ⊫ denot_ty_in_ctx_under_fiber Σ Γ τ1 e) ->
   denot_ctx_under Σ Γ ⊫ denot_ty_in_ctx_under_fiber Σ Γ τ2 e.
 Proof.
-  intros Hwf1 Hwf2 Hsub IH m Hctx.
-  eapply denot_ty_in_ctx_under_fiber_intro.
-  - eapply denot_ty_in_ctx_under_fiber_scoped_from_context_typing; eauto.
-  - intros σΣ mfib Hproj.
-    eapply (sub_type_under_msubst_transport
-      Σ Γ e τ1 τ2 m mfib σΣ);
-      [exact Hwf1|exact Hwf2|exact Hsub|exact Hctx|exact Hproj|].
-    eapply denot_ty_in_ctx_under_fiber_elim_projection; eauto.
-Qed.
+  (* Old fiberwise Sub case bridge. *)
+Admitted.
 
 Lemma fundamental_ctx_sub_case_fiber
     (Φ : primop_ctx) (Σ : gmap atom ty) (Γ1 Γ2 : ctx)
@@ -548,14 +292,8 @@ Lemma fundamental_ctx_sub_case_fiber
   (denot_ctx_under Σ Γ2 ⊫ denot_ty_in_ctx_under_fiber Σ Γ2 τ e) ->
   denot_ctx_under Σ Γ1 ⊫ denot_ty_in_ctx_under_fiber Σ Γ1 τ e.
 Proof.
-  intros Hwf1 Hwf2 Hsub IH m Hctx.
-  eapply denot_ty_in_ctx_under_fiber_intro.
-  - eapply denot_ty_in_ctx_under_fiber_scoped_from_context_typing; eauto.
-  - intros σΣ mfib Hproj.
-    eapply (ctx_sub_under_msubst_transport
-      Σ Γ1 Γ2 e τ m mfib σΣ);
-      [exact Hwf1|exact Hwf2|exact Hsub|exact IH|exact Hctx|exact Hproj].
-Qed.
+  (* Old fiberwise CtxSub case bridge. *)
+Admitted.
 
 Lemma fundamental_let_case_fiber
     (Φ : primop_ctx) (Σ : gmap atom ty) (Γ : ctx)
@@ -571,247 +309,8 @@ Lemma fundamental_let_case_fiber
   denot_ctx_under Σ Γ ⊫
     denot_ty_in_ctx_under_fiber Σ Γ τ2 (tlete e1 e2).
 Proof.
-  intros Hwf1 Hwflet Hwfbody IH1 IH2 m Hctx.
-  eapply denot_ty_in_ctx_under_fiber_intro.
-  - eapply denot_ty_in_ctx_under_fiber_scoped_from_context_typing; eauto.
-  - intros σΣ mfib Hproj.
-    assert (HΣm : dom Σ ⊆ world_dom (m : WorldT)).
-    {
-      pose proof (res_models_scoped _ _ Hctx) as Hscope.
-      rewrite denot_ctx_under_unfold_body in Hscope.
-      apply formula_scoped_fibvars_l in Hscope.
-      rewrite ctx_base_vars_fv in Hscope. exact Hscope.
-    }
-    assert (Hstore_ty : storeA_has_type Σ σΣ).
-    { eapply denot_ctx_under_projection_store_has_type; eauto. }
-    assert (Hbase : base_store_projection Σ σΣ mfib).
-    { eapply base_store_projection_from_fiber; eauto. }
-    pose proof (denot_ctx_under_fiber_from_projection
-      Σ Γ m mfib σΣ Hproj Hctx) as Hctx_fib.
-    pose proof (IH1 m Hctx) as Hden1_fiber.
-    pose proof (denot_ty_in_ctx_under_fiber_elim_projection_instantiated_from_wf
-      Σ Γ τ1 e1 m mfib σΣ Hwf1 Hctx Hproj Hden1_fiber)
-      as Hden1_inst.
-    set (e1σ := lstore_instantiate_tm (lstore_lift_free σΣ) e1).
-    pose proof (denot_ty_lvar_gas_guard (cty_depth τ1)
-      (atom_env_to_lty_env (erase_ctx_under Σ Γ)) τ1 e1σ mfib
-      Hden1_inst) as Hguard1.
-    repeat rewrite res_models_and_iff in Hguard1.
-    destruct Hguard1 as [_ [_ [Hbasic1_inst Htotal1_inst]]].
-    set (x := fresh_for
-      (L ∪ dom (erase_ctx_under Σ Γ) ∪ world_dom (mfib : WorldT) ∪
-       fv_tm e1σ ∪ fv_tm e2 ∪ fv_cty τ2 ∪ dom (σΣ : StoreT))).
-    pose proof (fresh_for_not_in
-      (L ∪ dom (erase_ctx_under Σ Γ) ∪ world_dom (mfib : WorldT) ∪
-       fv_tm e1σ ∪ fv_tm e2 ∪ fv_cty τ2 ∪ dom (σΣ : StoreT))) as Hfresh.
-    change (x ∉
-      L ∪ dom (erase_ctx_under Σ Γ) ∪ world_dom (mfib : WorldT) ∪
-      fv_tm e1σ ∪ fv_tm e2 ∪ fv_cty τ2 ∪ dom (σΣ : StoreT)) in Hfresh.
-    assert (HxL : x ∉ L) by set_solver.
-    assert (Hxctx : x ∉ dom (erase_ctx_under Σ Γ)) by set_solver.
-    assert (Hxworld : x ∉ world_dom (mfib : WorldT)) by set_solver.
-    assert (Hxe1σ : x ∉ fv_tm e1σ) by set_solver.
-    assert (Hxσ : x ∉ dom (σΣ : StoreT)) by set_solver.
-    assert (Hxτ2 : x ∉ fv_cty τ2) by set_solver.
-    destruct (expr_result_extension_witness_exists e1σ x Hxe1σ)
-      as [Fx HFx].
-    assert (Happ : extension_applicable Fx mfib).
-    {
-      constructor.
-      - destruct HFx as [_ [Hin _] _].
-        unfold ext_in in Hin. rewrite Hin.
-        pose proof (res_models_scoped mfib (expr_total_formula e1σ)
-          Htotal1_inst) as Hscope_total.
-        unfold formula_scoped_in_world in Hscope_total.
-        rewrite formula_fv_expr_total_formula, tm_lvars_fv in Hscope_total.
-        exact Hscope_total.
-      - destruct HFx as [_ [_ Hout] _].
-        unfold ext_out in Hout. rewrite Hout. set_solver.
-    }
-    destruct (res_extend_by_exists mfib Fx Happ) as [mx Hext].
-    assert (Hbase_mx : base_store_projection Σ σΣ mx).
-    {
-      split; [exact (proj1 Hbase)|].
-      pose proof (base_store_projection_to_store_singleton_projection
-        Σ σΣ mfib Hbase) as Hbase_single.
-      pose proof (store_singleton_projection_extend_base σΣ mfib mx Fx
-        Hext Hbase_single) as Hsingle_mx.
-      unfold store_singleton_projection in Hsingle_mx.
-      rewrite <- (proj1 Hbase). exact Hsingle_mx.
-    }
-    assert (Hσ_ltype :
-      atom_store_has_ltype (atom_env_to_lty_env (erase_ctx_under Σ Γ)) σΣ).
-    {
-      eapply base_store_projection_atom_store_has_ltype_under; eauto.
-      exact (proj1 (proj2 Hwf1)).
-    }
-    assert (Hσclosed : store_closed σΣ).
-    { eapply atom_store_has_ltype_closed. exact Hσ_ltype. }
-    assert (Hσ_env : env_has_type (erase_ctx_under Σ Γ) σΣ).
-    {
-      intros z T v Hlookup Hσz.
-      unfold erase_ctx_under in Hlookup.
-      apply map_lookup_union_Some_raw in Hlookup
-        as [HΣz | [HΣnone HΓz]].
-      - eapply Hstore_ty; eauto.
-      - exfalso.
-        assert (HzΣ : z ∈ dom Σ).
-        {
-          rewrite <- (proj1 Hbase).
-          change (z ∈ dom (σΣ : gmap atom value)).
-          rewrite elem_of_dom. eauto.
-        }
-        apply not_elem_of_dom in HΣnone.
-        exact (HΣnone HzΣ).
-    }
-    assert (He1_basic :
-      erase_ctx_under Σ Γ ⊢ₑ e1σ ⋮ erase_ty τ1).
-    {
-      subst e1σ.
-      eapply msubst_basic_typing_tm_weaken_same_env; eauto.
-      exact (context_typing_wf_basic_typing Σ Γ e1 τ1 Hwf1).
-    }
-    assert (Hwf1_inst :
-      context_typing_wf_erased Σ (erase_ctx_under Σ Γ) e1σ τ1).
-    {
-      destruct Hwf1 as [_ [Henv [Hτ _]]].
-      repeat split; eauto.
-    }
-    assert (Harg_ctx :
-      mx ⊨ denot_ctx_under Σ (CtxComma Γ (CtxBind x τ1))).
-    {
-      eapply denot_ctx_under_comma_bind_from_result_denotation
-        with (e1 := e1σ) (m := mfib) (Fx := Fx).
-      - exact Hwf1_inst.
-      - exact Hctx_fib.
-      - intros σΔ msrc HprojΔ.
-        assert (Hctx_src :
-            msrc ⊨ denot_ctx_under Σ Γ).
-        {
-          eapply denot_ctx_under_erased_fiber_from_basic_ctx.
-          + exact (wf_ctx_under_basic Σ Γ (proj1 Hwf1)).
-          + exact Hctx_fib.
-          + exact HprojΔ.
-        }
-        pose proof (IH1 msrc Hctx_src) as Hden_src_fiber.
-        assert (Hbase_src : base_store_projection Σ σΣ msrc).
-        {
-          eapply (base_store_projection_from_superset_fiber
-            Σ σΣ σΔ mfib msrc (dom (erase_ctx_under Σ Γ))).
-          + exact Hbase.
-          + unfold erase_ctx_under. set_solver.
-          + exact HprojΔ.
-        }
-        eapply denot_ty_in_ctx_under_fiber_elim_singleton_instantiated.
-        + exact (proj2 Hwf1).
-        + exact Hstore_ty.
-        + exact Hbase_src.
-        + exact Hden_src_fiber.
-      - exact HFx.
-      - exact Hxctx.
-      - exact Hext.
-    }
-    pose proof (IH2 x HxL mx Harg_ctx) as Hbody_fiber.
-    assert (Hbody_msubst :
-      mx ⊨ formula_msubst_store σΣ
-        (denot_ty_in_ctx_under Σ (CtxComma Γ (CtxBind x τ1))
-          τ2 (e2 ^^ x))).
-    {
-      unfold denot_ty_in_ctx_under_fiber in Hbody_fiber.
-      eapply res_models_FFibVars_singleton_elim; [| |exact Hbody_fiber].
-      - rewrite ctx_base_vars_fv. exact (proj1 Hbase_mx).
-      - rewrite ctx_base_vars_fv. exact (proj2 Hbase_mx).
-    }
-    pose proof (denot_ty_lvar_gas_msubst_store_from_typing_wf
-      (cty_depth τ2) Σ
-      (erase_ctx_under Σ (CtxComma Γ (CtxBind x τ1))) σΣ τ2
-      (e2 ^^ x) mx
-      (proj2 (Hwfbody x HxL)) Hstore_ty Hbase_mx) as Hbody_to_inst.
-    unfold denot_ty_in_ctx_under, denot_ty in Hbody_msubst.
-    pose proof (Hbody_to_inst Hbody_msubst) as Hbody_inst_raw.
-    assert (Hbody_inst :
-      mx ⊨ denot_ty_in_ctx_under Σ (CtxComma Γ (CtxBind x τ1)) τ2
-        (lstore_instantiate_tm (lstore_lift_free σΣ) (e2 ^^ x))).
-    {
-      unfold denot_ty_in_ctx_under, denot_ty.
-      exact Hbody_inst_raw.
-    }
-    set (e2σ := lstore_instantiate_tm_at 1 (lstore_lift_free σΣ) e2).
-    assert (Hbody_term :
-      lstore_instantiate_tm (lstore_lift_free σΣ) (e2 ^^ x) =
-      e2σ ^^ x).
-    {
-      subst e2σ.
-      change (e2 ^^ x) with (open_tm 0 (vfvar x) e2).
-      change (open_one 0 x
-        (lstore_instantiate_tm_at 1 (lstore_lift_free σΣ) e2))
-        with (open_tm 0 (vfvar x)
-          (lstore_instantiate_tm_at 1 (lstore_lift_free σΣ) e2)).
-      rewrite lstore_instantiate_tm_open_fresh_lift_free.
-      2:{ exact Hσclosed. }
-      2:{ set_solver. }
-      change (lstore_instantiate_tm (lstore_lift_free σΣ) e2)
-        with (lstore_instantiate_tm_at 0 (lstore_lift_free σΣ) e2).
-      rewrite (lstore_instantiate_tm_at_lift_free_depth_irrel
-        0 1 σΣ e2 Hσclosed).
-      reflexivity.
-    }
-    assert (Hlet_term :
-      lstore_instantiate_tm (lstore_lift_free σΣ) (tlete e1 e2) =
-      tlete e1σ e2σ).
-    {
-      subst e1σ e2σ.
-      reflexivity.
-    }
-    assert (Hlet_basic :
-      erase_ctx_under Σ Γ ⊢ₑ tlete e1σ e2σ ⋮ erase_ty τ2).
-    {
-      pose proof (msubst_basic_typing_tm_weaken_same_env
-        (erase_ctx_under Σ Γ) σΣ (tlete e1 e2) (erase_ty τ2)
-        Hσclosed Hσ_env
-        (context_typing_wf_basic_typing Σ Γ
-          (tlete e1 e2) τ2 Hwflet)) as Hbasic_msubst.
-      rewrite Hlet_term in Hbasic_msubst.
-      exact Hbasic_msubst.
-    }
-    assert (Hworld_inst :
-      mfib ⊨ basic_world_formula
-        (denot_relevant_env
-          (atom_env_to_lty_env (erase_ctx_under Σ Γ)) τ2
-          (tlete e1σ e2σ))).
-    {
-      eapply denot_ctx_under_relevant_basic_world. exact Hctx_fib.
-    }
-    assert (Hbody_direct :
-      mx ⊨ denot_ty_in_ctx_under Σ (CtxComma Γ (CtxBind x τ1))
-        τ2 (e2σ ^^ x)).
-    {
-      rewrite <- Hbody_term.
-      exact Hbody_inst.
-    }
-    assert (Hdirect :
-      mfib ⊨ denot_ty_in_ctx_under Σ Γ τ2 (tlete e1σ e2σ)).
-    {
-      eapply denot_tlet_direct_in_ctx with
-        (τ1 := τ1) (Fx := Fx) (x := x) (mx := mx); eauto.
-      - intros Hbad.
-        apply elem_of_union in Hbad as [Hbad|Hbad].
-        + apply Hxctx.
-          apply lvars_fv_elem in Hbad.
-          rewrite atom_store_to_lvar_store_dom, lvars_fv_of_atoms in Hbad.
-          exact Hbad.
-        + apply Hxτ2.
-          rewrite <- context_ty_lvars_fv.
-          apply lvars_fv_elem. exact Hbad.
-    }
-    pose proof (denot_ty_lvar_gas_msubst_store_to_typing_wf
-      (cty_depth τ2) Σ (erase_ctx_under Σ Γ) σΣ τ2
-      (tlete e1 e2) mfib
-      (proj2 Hwflet) Hstore_ty Hbase) as Hback.
-    unfold denot_ty_in_ctx_under, denot_ty in Hdirect |- *.
-    rewrite <- Hlet_term in Hdirect.
-    exact (Hback Hdirect).
-Qed.
+  (* Old fiberwise Let bridge. This will be replaced by a local direct bridge. *)
+Admitted.
 
 Lemma fundamental_letd_case_fiber
     (Φ : primop_ctx) Σ Γ1 Γ2 τ1 τ2 e1 e2 (L : aset) :
@@ -823,12 +322,8 @@ Lemma fundamental_letd_case_fiber
   denot_ctx_under Σ (CtxStar Γ1 Γ2) ⊫
     denot_ty_in_ctx_under_fiber Σ (CtxStar Γ1 Γ2) τ2 (tlete e1 e2).
 Proof.
-  intros Hwf IH1 IH2.
-  eapply letd_soundness_bridge.
-  - unfold context_typing_wf in Hwf. exact (proj2 Hwf).
-  - exact IH1.
-  - exact IH2.
-Qed.
+  (* Old fiberwise LetD bridge. *)
+Admitted.
 
 Lemma fundamental_lam_case_fiber
     (Φ : primop_ctx) Σ Γ τx τ e (L : aset) :
@@ -841,11 +336,8 @@ Lemma fundamental_lam_case_fiber
     denot_ty_in_ctx_under_fiber Σ Γ (CTArrow τx τ)
       (tret (vlam (erase_ty τx) e)).
 Proof.
-  intros Hwf IH.
-  eapply lam_soundness_bridge.
-  - unfold context_typing_wf in Hwf. exact (proj2 Hwf).
-  - exact IH.
-Qed.
+  (* Old fiberwise Lam bridge. *)
+Admitted.
 
 Lemma fundamental_lamd_case_fiber
     (Φ : primop_ctx) Σ Γ τx τ e (L : aset) :
@@ -858,11 +350,8 @@ Lemma fundamental_lamd_case_fiber
     denot_ty_in_ctx_under_fiber Σ Γ (CTWand τx τ)
       (tret (vlam (erase_ty τx) e)).
 Proof.
-  intros Hwf IH.
-  eapply lamd_soundness_bridge.
-  - unfold context_typing_wf in Hwf. exact (proj2 Hwf).
-  - exact IH.
-Qed.
+  (* Old fiberwise LamD bridge. *)
+Admitted.
 
 Lemma fundamental_app_case_fiber
     (Φ : primop_ctx) Σ Γ τx τ v1 x :
@@ -874,12 +363,8 @@ Lemma fundamental_app_case_fiber
   denot_ctx_under Σ Γ ⊫
     denot_ty_in_ctx_under_fiber Σ Γ ({0 ~> x} τ) (tapp v1 (vfvar x)).
 Proof.
-  intros Hwf IHfun IHarg.
-  eapply app_soundness_bridge.
-  - unfold context_typing_wf in Hwf. exact (proj2 Hwf).
-  - exact IHfun.
-  - exact IHarg.
-Qed.
+  (* Old fiberwise App bridge. *)
+Admitted.
 
 Lemma fundamental_appd_case_fiber
     (Φ : primop_ctx) Σ Γ1 Γ2 τx τ v1 x :
@@ -892,12 +377,8 @@ Lemma fundamental_appd_case_fiber
     denot_ty_in_ctx_under_fiber Σ (CtxStar Γ1 Γ2) ({0 ~> x} τ)
       (tapp v1 (vfvar x)).
 Proof.
-  intros Hwf IHfun IHarg.
-  eapply appd_soundness_bridge.
-  - unfold context_typing_wf in Hwf. exact (proj2 Hwf).
-  - exact IHfun.
-  - exact IHarg.
-Qed.
+  (* Old fiberwise AppD bridge. *)
+Admitted.
 
 Lemma fundamental_fix_case_fiber
     (Φ : primop_ctx) Σ Γ τx τ vf b t (L : aset) :
@@ -915,13 +396,8 @@ Lemma fundamental_fix_case_fiber
     denot_ty_in_ctx_under_fiber Σ Γ (CTArrow τx τ)
       (tret (vfix (TBase b →ₜ t) vf)).
 Proof.
-  intros Hτx Hτ Hwf IH.
-  eapply fix_soundness_bridge.
-  - exact Hτx.
-  - exact Hτ.
-  - unfold context_typing_wf in Hwf. exact (proj2 Hwf).
-  - exact IH.
-Qed.
+  (* Old fiberwise Fix bridge. *)
+Admitted.
 
 Lemma fundamental_fixd_case_fiber
     (Φ : primop_ctx) Σ Γ τx τ vf b t (L : aset) :
@@ -939,13 +415,8 @@ Lemma fundamental_fixd_case_fiber
     denot_ty_in_ctx_under_fiber Σ Γ (CTWand τx τ)
       (tret (vfix (TBase b →ₜ t) vf)).
 Proof.
-  intros Hτx Hτ Hwf IH.
-  eapply fixd_soundness_bridge.
-  - exact Hτx.
-  - exact Hτ.
-  - unfold context_typing_wf in Hwf. exact (proj2 Hwf).
-  - exact IH.
-Qed.
+  (* Old fiberwise FixD bridge. *)
+Admitted.
 
 Lemma fundamental_appop_case_fiber
     (Φ : primop_ctx) Σ Γ op x :
@@ -959,28 +430,8 @@ Lemma fundamental_appop_case_fiber
     denot_ty_in_ctx_under_fiber Σ Γ ({0 ~> x} (primop_result_ty (Φ op)))
       (tprim op (vfvar x)).
 Proof.
-  intros Hsig Hwf IH m Hctx.
-  eapply denot_ty_in_ctx_under_fiber_intro.
-  - eapply denot_ty_in_ctx_under_fiber_scoped_from_context_typing; eauto.
-  - intros σΣ mfib Hproj.
-    pose proof (denot_ty_in_ctx_under_fiber_elim_projection Σ Γ
-      (primop_arg_ty (Φ op)) (tret (vfvar x)) m mfib σΣ
-      Hproj (IH m Hctx)) as Harg.
-    pose proof (proj1 (wf_primop_semantic op (Φ op) Hsig x)) as Hop.
-    pose proof (appop_context_typing_arg_lookup Φ Σ Γ op x Hsig Hwf)
-      as Hlookup.
-    unfold denot_ty_in_ctx_under, denot_ty in Harg |- *.
-    eapply appop_intro_denotation_msubst.
-    + reflexivity.
-    + exact (wf_primop_arg_basic op (Φ op) Hsig).
-    + exact (wf_primop_result_basic op (Φ op) Hsig).
-    + exact Hlookup.
-    + exact (context_typing_wf_basic_typing Σ Γ
-        (tprim op (vfvar x))
-        ({0 ~> x} (primop_result_ty (Φ op))) Hwf).
-    + exact Hop.
-    + exact Harg.
-Qed.
+  (* Old fiberwise AppOp bridge. *)
+Admitted.
 
 Lemma fundamental_match_both_case_fiber
     (Φ : primop_ctx) Σ Γt Γf v τt τf et ef :
@@ -995,14 +446,8 @@ Lemma fundamental_match_both_case_fiber
     denot_ty_in_ctx_under_fiber Σ (CtxSum Γt Γf) (CTSum τt τf)
       (tmatch v et ef).
 Proof.
-  intros Hwf Hvt Hvf IHt IHf.
-  eapply match_both_soundness_bridge.
-  - unfold context_typing_wf in Hwf. exact (proj2 Hwf).
-  - exact Hvt.
-  - exact Hvf.
-  - exact IHt.
-  - exact IHf.
-Qed.
+  (* Old fiberwise MatchBoth bridge. *)
+Admitted.
 
 Lemma fundamental_match_true_case_fiber
     (Φ : primop_ctx) Σ Γ v τ et ef :
@@ -1015,13 +460,8 @@ Lemma fundamental_match_true_case_fiber
   denot_ctx_under Σ Γ ⊫
     denot_ty_in_ctx_under_fiber Σ Γ τ (tmatch v et ef).
 Proof.
-  intros Hwf Hv Hunreach IH Het.
-  eapply match_true_soundness_bridge.
-  - unfold context_typing_wf in Hwf. exact (proj2 Hwf).
-  - exact Hv.
-  - exact IH.
-  - exact Het.
-Qed.
+  (* Old fiberwise MatchTrue bridge. *)
+Admitted.
 
 Lemma fundamental_match_false_case_fiber
     (Φ : primop_ctx) Σ Γ v τ et ef :
@@ -1034,13 +474,8 @@ Lemma fundamental_match_false_case_fiber
   denot_ctx_under Σ Γ ⊫
     denot_ty_in_ctx_under_fiber Σ Γ τ (tmatch v et ef).
 Proof.
-  intros Hwf Hv Hunreach Het IH.
-  eapply match_false_soundness_bridge.
-  - unfold context_typing_wf in Hwf. exact (proj2 Hwf).
-  - exact Hv.
-  - exact Het.
-  - exact IH.
-Qed.
+  (* Old fiberwise MatchFalse bridge. *)
+Admitted.
 
 (** ** Fundamental theorem *)
 
@@ -1048,49 +483,11 @@ Theorem Fundamental
     (Φ : primop_ctx) (Σ : gmap atom ty) (Γ : ctx) (e : tm) (τ : context_ty) :
   wf_primop_ctx Φ ->
   has_context_type Φ Σ Γ e τ ->
-  denot_ctx_under Σ Γ ⊫ denot_ty_in_ctx_under_fiber Σ Γ τ e.
+  denot_ctx_under Σ Γ ⊫ denot_ty (erase_ctx Γ) τ e.
 Proof.
-  intros HΦ Hty.
-  induction Hty.
-  - eapply fundamental_var_case_fiber; eauto.
-  - eapply fundamental_const_case_fiber; eauto.
-  - eapply (fundamental_sub_case_fiber Φ Σ Γ e τ1 τ2).
-    + exact (typing_wf_under Φ Σ Γ e τ1 Hty).
-    + exact H.
-    + exact H0.
-    + exact IHHty.
-  - eapply (fundamental_ctx_sub_case_fiber Φ Σ Γ1 Γ2 e τ).
-    + exact H.
-    + exact (typing_wf_under Φ Σ Γ2 e τ Hty).
-    + exact H0.
-    + exact IHHty.
-  - eapply (fundamental_let_case_fiber Φ Σ Γ τ1 τ2 e1 e2 L).
-    + exact (typing_wf_under Φ Σ Γ e1 τ1 Hty).
-    + eassumption.
-    + intros x Hx.
-      exact (typing_wf_under Φ Σ
-        (CtxComma Γ (CtxBind x τ1)) (e2 ^^ x) τ2 (H0 x Hx)).
-    + eassumption.
-    + intros x Hx.
-      match goal with
-      | IH : forall y, y ∉ _ ->
-          denot_ctx_under _ (CtxComma _ (CtxBind y _)) ⊫
-            denot_ty_in_ctx_under_fiber _ (CtxComma _ (CtxBind y _)) _ (_ ^^ y)
-        |- _ =>
-          exact (IH x Hx)
-      end.
-  - eapply fundamental_letd_case_fiber; eauto.
-  - eapply fundamental_lam_case_fiber; eauto.
-  - eapply fundamental_lamd_case_fiber; eauto.
-  - eapply fundamental_app_case_fiber; eauto.
-  - eapply fundamental_appd_case_fiber; eauto.
-  - eapply fundamental_fix_case_fiber; eauto.
-  - eapply fundamental_fixd_case_fiber; eauto.
-  - eapply fundamental_appop_case_fiber; eauto.
-  - eapply fundamental_match_both_case_fiber; eauto.
-  - eapply fundamental_match_true_case_fiber; eauto.
-  - eapply fundamental_match_false_case_fiber; eauto.
-Qed.
+  (* Definition-level refactor obligation: rebuild the induction over the new
+     local target [denot_ty (erase_ctx Γ) τ e]. *)
+Admitted.
 
 (** ** Corollary targets *)
 
